upcasting certificate chains to TLS 1.3

src/tls/Extensions.fst
@@ -246,7 +246,7 @@ noeq type extension =
   | E_supported_groups of list namedGroup (* M, AF *) (* RFC 7919 *)  
   | E_signature_algorithms of (list sigHashAlg) (* M, AF *) (* RFC 5246 *)
   | E_key_share of CommonDH.keyShare (* M, AF *)
-  | E_pre_shared_key of (list psk) (* M, AF *)
+  | E_pre_shared_key of list psk (* M, AF *)
   | E_early_data of earlyDataIndication
   | E_supported_versions of protocol_versions   (* M, AF *) 
   | E_cookie of b:bytes {0 < length b /\ length b < 65536}  (* M *)
@@ -358,22 +358,46 @@ let rec extensionBytes ext =
   let payload = vlbytes 2 payload in
   head @| payload
 
-type extensions = 
-  exts:list extension {repr_bytes (length (List.Tot.fold_left (fun l s -> l @| extensionBytes s) empty_bytes exts)) <= 2}
+val extensionListBytes: exts: list extension -> bytes 
+let extensionListBytes exts = List.Tot.fold_left (fun l s -> l @| extensionBytes s) empty_bytes exts
 
+type extensions = exts:list extension {repr_bytes (length (extensionListBytes exts)) <= 2}
+
+val noExtensions: exts:extensions {exts == []}
+let noExtensions = 
+  lemma_repr_bytes_values (length (extensionListBytes [])); 
+  []
+  
 val extensionsBytes: extensions -> b:bytes { length b < 2 + 65536 }
 let extensionsBytes exts =
-  let b = List.Tot.fold_left (fun l s -> l @| extensionBytes s) empty_bytes exts in
+  let b = extensionListBytes exts in
   lemma_repr_bytes_values (length b);
   vlbytes 2 b
 
+
+(* CERTIFICATES (relocate?)  
+
+The chain format changes between TLS 1.2 and TLS 1.3; we separate then
+in messages, but at least for now, we merge the two in Negotiation and
+in the main TLS API (with no extensions when using TLS 1.2 *)
+
 // opaque cert_data<1..2^24-1>
 type cert = b:bytes {length b < 16777216}
-
+type certes = cert * extensions
 // CertificateEntry certificate_list<0..2^24-1>;
 // See https://tlswg.github.io/tls13-spec/#rfc.section.4.4.2
 type chain = l:list cert // { ... }
-type chain13 = l:list (cert * extensions) // { ... }
+type chain13 = l:list certes // { ... }
+
+// we may use these types to keep track of un-extended chains, 
+// e.g. to prove that their formatting is injective
+let is_classic_chain (l:chain13): bool = 
+  List.Tot.for_all #certes (fun ces -> List.Tot.isEmpty (snd ces)) l
+type chain12 = l:chain13 {is_classic_chain l}  
+
+// todo: prove it is a chain12
+let chain_up (l:chain): chain13= List.Tot.map #cert #certes (fun c -> c,[]) l 
+let chain_down (l:chain13): chain = List.Tot.map #certes #cert fst l
 
 
 (*************************************************
